\newproblem{11a}
{
	Solve for $w$ and be sure to simplify your answer.
	
	$\displaystyle \frac{3}{4}w-3=\frac{1}{2}w+2$
}
{
	\begin{tabular}{l r}
	$(4)\frac{3}{4}w-(4)3=(4)\frac{1}{2}w+(4)2$ & 2 pts to here\\
	$3w-12=2w+8$ & 4 pts to here\\
	$w-12=8$ & 6 pts to here\\
	$w=20$ & 8 pts to here
	\end{tabular}
}

\newproblem{11b}
{
	Solve for $w$ and be sure to simplify your answer.
	
	$\displaystyle \frac{5}{4}w-1=\frac{3}{4}w +\frac{1}{2}$
}
{
	\begin{tabular}{l r}
	$(4)\frac{5}{4}w-1(4)=(4)\frac{3}{4}w +(4)\frac{1}{2}$ & 2 pts to here\\
	$5w-4=3w+2$ & 4 pts to here\\
	$2w=6$ & 6 pts to here\\
	$w=3$ & 8 pts to here
	\end{tabular}
}

\newproblem{11c}
{
	Solve for $w$ and be sure to simplify your answer.
	
	$\displaystyle \frac{1}{3}w+3=\frac{1}{5}w -\frac{1}{3}$
}
{
	\begin{tabular}{l r}
	$(15)\frac{1}{3}w+3(15)=(15)\frac{1}{5}w +(15)\frac{1}{3}$ & 2 pts to here\\
	$5w+45=3w-5$ & 4 pts to here\\
	$2w=-50$ & 6 pts to here\\
	$w=-25$ & 8 pts to here
	\end{tabular}
}

\newproblem{11d}
{
	Solve for $w$ and be sure to simplify your answer.
	
	$\displaystyle \frac{1}{4}w+\frac{1}{2}=w -\frac{7}{4}$
}
{
	\begin{tabular}{l r}
	$(4)\frac{1}{4}w+(4)\frac{1}{2}=4w -(4)\frac{7}{4}$ & 2 pts to here\\
	$w+2=4w-7$ & 4 pts to here\\
	$-3w=-9$ & 6 pts to here\\
	$w=3$ & 8 pts to here
	\end{tabular}
}
